LeanSubst/Laws.lean
@@ -16,253 +16,255 @@ theorem Ren.lift_eq_from_eq [RenMap T [T]] {r : Ren T} {σ : Subst T}
   : r.to = σ -> r.to.lift = σ.lift
 := by intro h; rw [<-h]
 
--- namespace Subst
---   section
---     @[simp]
---     theorem rewrite0 [RenMap T [T]] : +0σ ∘ +1r = succ T := by
---       congr
+namespace Subst
+  section
+    @[simp]
+    theorem rewrite0 [RenMap T [T]] : +0σ ∘ +1r = succ T := by
+      congr
 
---     @[simp, grind =]
---     theorem rewrite1 : re 0 :: +1σ = id T := by
---       simp [Subst.cons, Subst.id]
---       funext; case _ x =>
---       cases x; all_goals simp
+    @[simp, grind =]
+    theorem rewrite1 : re 0 :: +1σ = id T := by
+      simp [Subst.cons, Subst.id]
+      funext; case _ x =>
+      cases x; all_goals simp
 
---     @[simp, grind =]
---     theorem rewrite1_ren : 0 :: +1r = Ren.id T := by
---       simp [Ren.cons, Ren.id]
---       funext; case _ x =>
---       cases x <;> simp
+    @[simp, grind =]
+    theorem rewrite1_ren : 0 :: +1r = Ren.id T := by
+      simp [Ren.cons, Ren.id]
+      funext; case _ x =>
+      cases x <;> simp
 
---     open SubstMap
+    open SubstMap
 
---     @[simp, grind =]
---     theorem I_lift [RenMap T [T]] {k} : +0σ.lift k = id T := by
---       funext; case _ x =>
---       cases x; all_goals (simp [lift, id, act, SubstAction.act])
---       sorry --grind
+    @[simp, grind =]
+    theorem I_lift [RenMap T [T]] {k} : +0σ.lift k = id T := by
+      funext; case _ x =>
+      cases x; all_goals (simp [lift, id, act, SubstAction.act])
+      grind
 
---     @[simp, grind =]
---     theorem rewrite2 [SubstMap T [T]] {σ : Subst T} : +0σ ∘ σ = σ := by
---       funext; case _ x =>
---       simp [compose, id, act, SubstAction.act]
---       sorry
+    @[simp, grind =]
+    theorem rewrite2 [SubstMap T [T]] {σ : Subst T} : +0σ ∘ σ = σ := by
+      funext; case _ x =>
+      simp [compose, id, act, SubstAction.act]
 
---     @[simp, grind =]
---     theorem rewrite2_ren [SubstMap T [T]] {σ : Subst T} : +0r ∘ σ = σ := by
---       funext; case _ x =>
---       simp [compose_ren_left, act, SubstAction.act]
+    @[simp, grind =]
+    theorem rewrite2_ren [SubstMap T [T]] {σ : Subst T} : +0r ∘ σ = σ := by
+      funext; case _ x =>
+      simp [compose_ren_left, act, SubstAction.act]
 
---     @[simp, grind =]
---     theorem rewrite3_cons [SubstMap T [T]] {σ τ : Subst T} {a : Action T}
---       : (a :: σ) ∘ τ = a[τ] :: (σ ∘ τ)
---     := by
---       simp [cons, compose]
---       funext; case _ x =>
---       cases x; all_goals simp [act, SubstAction.act]
+    @[simp, grind =]
+    theorem rewrite3_cons [SubstMap T [T]] {σ τ : Subst T} {a : Action T}
+      : (a :: σ) ∘ τ = a[τ] :: (σ ∘ τ)
+    := by
+      simp [cons, compose]
+      funext; case _ x =>
+      cases x; all_goals simp [act, SubstAction.act]
 
---     @[simp, grind =]
---     theorem rewrite3_cons_ren [RenMap T [T]] [SubstMap T [T]] {σ : Subst T} {r : Ren T} {x : Nat}
---       : (re x :: σ) ∘ r = re (r.act x) :: (σ ∘ r)
---     := by
---       simp [cons, compose_ren_right]
---       funext; case _ x =>
---       cases x; sorry; all_goals simp [act, SubstAction.act]
+    @[simp, grind =]
+    theorem rewrite3_cons_ren [RenMap T [T]] [SubstMap T [T]] {σ : Subst T} {r : Ren T} {x : Nat}
+      : (re x :: σ) ∘ r = re (r.act x) :: (σ ∘ r)
+    := by
+      simp [cons, compose_ren_right]
+      funext; case _ x =>
+      cases x; all_goals simp [act, SubstAction.act]
 
-  --   @[simp, grind =]
-  --   theorem rewrite3_append [SubstMap T [T]] {σ τ : Subst T} {ℓ : List (Action T)}
-  --     : (ℓ ++ σ) ∘ τ = ℓ[τ] ++ (σ ∘ τ)
-  --   := by
-  --     induction ℓ generalizing σ τ <;> simp
-  --     case _ hd tl ih =>
-  --     cases hd <;> simp [*]
+    @[simp, grind =]
+    theorem rewrite3_append [SubstMap T [T]] {σ τ : Subst T} {ℓ : List (Action T)}
+      : (ℓ ++ σ) ∘ τ = ℓ[τ] ++ (σ ∘ τ)
+    := by
+      induction ℓ generalizing σ τ <;> simp
+      case _ hd tl ih =>
+      cases hd <;> simp [*]
 
-  --   @[simp, grind =]
-  --   theorem rewrite3_append_act [SubstMap T [T]] {σ τ : Subst T} {ℓ : List Nat}
-  --     : (ℓ ++ σ) ∘ τ = τ.act ℓ ++ (σ ∘ τ)
-  --   := by induction ℓ generalizing σ τ <;> simp [*]
+    @[simp, grind =]
+    theorem rewrite3_append_act [SubstMap T [T]] {σ τ : Subst T} {ℓ : List Nat}
+      : (ℓ ++ σ) ∘ τ = τ.act ℓ ++ (σ ∘ τ)
+    := by induction ℓ generalizing σ τ <;> simp [*]
 
-  --   @[simp, grind =]
-  --   theorem rewrite3_append_ren [RenMap T [T]] [SubstMap T [T]] {σ : Subst T} {r : Ren T} {ℓ : List Nat}
-  --     : (ℓ ++ σ) ∘ r = ℓ⟨r⟩ ++ (σ ∘ r)
-  --   := by
-  --     induction ℓ generalizing σ r <;> simp
-  --     case _ hd tl ih =>
-  --     cases hd <;> simp [*]
+    @[simp, grind =]
+    theorem rewrite3_append_ren [RenMap T [T]] [SubstMap T [T]] {σ : Subst T} {r : Ren T} {ℓ : List Nat}
+      : (ℓ ++ σ) ∘ r = ℓ⟨r⟩ ++ (σ ∘ r)
+    := by
+      induction ℓ generalizing σ r <;> simp
+      case _ hd tl ih =>
+      cases hd <;> simp [*]
 
-  --   @[simp, grind =]
-  --   theorem rewrite4_cons [SubstMap T [T]]  {s} {σ : Subst T} : +1σ ∘ (s :: σ) = σ := by
-  --     simp [Subst.cons]
-  --     funext; case _ x =>
-  --     cases x; all_goals (simp [compose, succ, act, SubstAction.act])
+    @[simp, grind =]
+    theorem rewrite4_cons [SubstMap T [T]]  {s} {σ : Subst T} : +1σ ∘ (s :: σ) = σ := by
+      simp [Subst.cons]
+      funext; case _ x =>
+      cases x; all_goals (simp [compose, succ, act, SubstAction.act])
 
-  --   @[simp, grind =]
-  --   theorem rewrite4_cons_ren [SubstMap T [T]]  {s} {σ : Subst T} : +1r ∘ (s :: σ) = σ := by
-  --     simp [Subst.cons]
-  --     funext; case _ x =>
-  --     cases x; all_goals (simp [compose_ren_left, act, SubstAction.act])
+    @[simp, grind =]
+    theorem rewrite4_cons_ren [SubstMap T [T]]  {s} {σ : Subst T} : +1r ∘ (s :: σ) = σ := by
+      simp [Subst.cons]
+      funext; case _ x =>
+      cases x; all_goals (simp [compose_ren_left, act, SubstAction.act])
 
-  --   @[simp, grind =]
-  --   theorem rewrite5 [SubstMap T [T]] {σ : Subst T} : σ.act 0 :: (+1σ ∘ σ) = σ := by
-  --     simp [Subst.cons, Subst.compose]; congr
-  --     funext; case _ x =>
-  --     cases x <;> simp [act, SubstAction.act]
+    @[simp, grind =]
+    theorem rewrite5 [SubstMap T [T]] {σ : Subst T} : σ.act 0 :: (+1σ ∘ σ) = σ := by
+      simp [Subst.cons, Subst.compose]; congr
+      funext; case _ x =>
+      cases x <;> simp [act, SubstAction.act]
 
-  --   @[simp, grind =]
-  --   theorem rewrite5_ren [SubstMap T [T]] {σ : Subst T} : σ.act 0 :: (+1r ∘ σ) = σ := by
-  --     simp [Subst.cons]; congr
-  --     funext; case _ x =>
-  --     cases x <;> simp [act, SubstAction.act]
-  -- end
+    @[simp, grind =]
+    theorem rewrite5_ren [SubstMap T [T]] {σ : Subst T} : σ.act 0 :: (+1r ∘ σ) = σ := by
+      simp [Subst.cons]; congr
+      funext; case _ x =>
+      cases x <;> simp [act, SubstAction.act]
+  end
 
-  -- @[simp, grind =]
-  -- theorem rewrite_lift [RenMap T [T]] {σ : Subst T}
-  --   : σ.lift = re 0 :: (σ ∘ +1r)
-  -- := by
-  --   simp [cons, lift, compose_ren_right]
-  --   funext; case _ x =>
-  --   cases x <;> simp
+  @[simp, grind =]
+  theorem rewrite_lift [RenMap T [T]] {σ : Subst T}
+    : σ.lift = re 0 :: (σ ∘ +1r)
+  := by
+    simp [cons, lift, compose_ren_right]
+    funext; case _ x =>
+    cases x <;> simp
 
-  -- @[simp, grind =]
-  -- theorem rewrite_lift_zero [RenMap T [T]] [RenMapId T T] {σ : Subst T}
-  --   : σ.lift 0 = σ
-  -- := by simp [lift, act, SubstAction.act]
+  @[simp, grind =]
+  theorem rewrite_lift_zero [RenMap T [T]] [RenMapId T [T]] {σ : Subst T}
+    : σ.lift 0 = σ
+  := by
+    simp [lift, act, SubstAction.act]
 
-  -- @[grind =]
-  -- theorem rewrite_lift_succ
-  --   [RenMap T [T]] [RenMapId T T] [RenMapCompose T T]
-  --   {k} {σ : Subst T}
-  --   : σ.lift (k + 1) = (σ.lift k).lift
-  -- := by
-  --   induction k; simp
-  --   case _ n ih =>
-  --     replace ih (i : Nat) : (σ.lift (n + 1)).act i = ((σ.lift n).lift 1).act i := by rw [ih]
-  --     simp [Subst.lift]
-  --     funext; case _ i =>
-  --     have lem := ih i
-  --     cases i <;> simp [act, SubstAction.act]
-  --     case _ k =>
-  --     split <;> simp
-  --     rw [Ren.compose_add_succ_right]
+  @[grind =]
+  theorem rewrite_lift_succ
+    [RenMap T [T]] [RenMapId T [T]] [RenMapCompose T [T]]
+    {k} {σ : Subst T}
+    : σ.lift (k + 1) = (σ.lift k).lift
+  := by
+    induction k; simp
+    case _ n ih =>
+      replace ih (i : Nat) : (σ.lift (n + 1)).act i = ((σ.lift n).lift 1).act i := by rw [ih]
+      simp [Subst.lift]
+      funext; case _ i =>
+      have lem := ih i
+      cases i <;> simp [act, SubstAction.act]
+      sorry
+      -- case _ k =>
+      -- split <;> simp
+      -- rw [Ren.compose_add_succ_right]
 
-  -- @[simp, grind =]
-  -- theorem rewrite6 [RenMap T [T]] [SubstMap T [T]] [SubstMapId T T] {σ : Subst T}
-  --   : σ ∘ +0σ = σ
-  -- := by
-  --   simp [compose, id, act, SubstAction.act]; congr; funext; case _ x =>
-  --   generalize zdef : σ.inner x = z
-  --   cases z <;> simp [act, SubstAction.act]
-  --   case _ t =>
-  --   have lem : t[id T] = t := by simp
-  --   simp [id] at lem; exact lem
+  @[simp, grind =]
+  theorem rewrite6 [RenMap T [T]] [SubstMap T [T]] [SubstMapId T [T]] {σ : Subst T}
+    : σ ∘ +0σ = σ
+  := by
+    simp [compose, id, act, SubstAction.act]; congr; funext; case _ x =>
+    generalize zdef : σ.inner x = z
+    cases z <;> simp [act, SubstAction.act]
+    case _ t =>
+    have lem : t[id T] = t := by simp
+    simp [id] at lem; exact lem
 
-  -- @[simp, grind =]
-  -- theorem rewrite6_ren [RenMap T [T]] [RenMapId T T] {σ : Subst T}
-  --   : σ ∘ +0r = σ
-  -- := by
-  --   simp [compose_ren_right]; congr
+  @[simp, grind =]
+  theorem rewrite6_ren [RenMap T [T]] [RenMapId T [T]] {σ : Subst T}
+    : σ ∘ +0r = σ
+  := by
+    simp [compose_ren_right]; congr
 
-  -- @[simp, grind =]
-  -- theorem rewrite7
-  --   [SubstMap T [T]] [SubstMapCompose T T]
-  --   {σ τ μ : Subst T}
-  --   : (σ ∘ τ) ∘ μ = σ ∘ τ ∘ μ
-  -- := by
-  --   simp [Subst.compose, act, SubstAction.act]
-  --   funext; case _ x =>
-  --   cases σ.inner x <;> simp [act, SubstAction.act]
-  --   simp [compose, act, SubstAction.act]
+  @[simp, grind =]
+  theorem rewrite7
+    [SubstMap T [T]] [SubstMapCompose T [T]]
+    {σ τ μ : Subst T}
+    : (σ ∘ τ) ∘ μ = σ ∘ τ ∘ μ
+  := by
+    simp [Subst.compose, act, SubstAction.act]
+    funext; case _ x =>
+    cases σ.inner x <;> simp [act, SubstAction.act]
+    simp [compose_tuple, compose, act, SubstAction.act]
+    congr
 
-  -- @[simp, grind =]
-  -- theorem rewrite7_ren
-  --   [RenMap T [T]] [RenMapCompose T T]
-  --   {σ : Subst T} {r1 r2 : Ren T}
-  --   : (σ ∘ r1) ∘ r2 = σ ∘ r1 ∘ r2
-  -- := by simp [compose_ren_right]
+  @[simp, grind =]
+  theorem rewrite7_ren
+    [RenMap T [T]] [RenMapCompose T [T]]
+    {σ : Subst T} {r1 r2 : Ren T}
+    : (σ ∘ r1) ∘ r2 = σ ∘ r1 ∘ r2
+  := by simp [compose_ren_right, Ren.compose_tuple]
 
-  -- @[simp, grind =]
-  -- theorem rewrite4_append_direct [SubstMap T [T]] [SubstMapCompose T T]
-  --   {ℓ : List $ Action T} {σ : Subst T}
-  --   : (add T ℓ.length) ∘ (ℓ ++ σ) = σ
-  -- := by
-  --   induction ℓ generalizing σ <;> simp
-  --   case _ hd tl ih =>
-  --   rw [compose_add_succ_right]
-  --   simp [*]
+  @[simp, grind =]
+  theorem rewrite4_append_direct [SubstMap T [T]] [SubstMapCompose T [T]]
+    {ℓ : List $ Action T} {σ : Subst T}
+    : (add T ℓ.length) ∘ (ℓ ++ σ) = σ
+  := by
+    induction ℓ generalizing σ <;> simp
+    case _ hd tl ih =>
+    rw [compose_add_succ_right]
+    simp [*]
 
-  -- @[simp, grind <-]
-  -- theorem rewrite4_append_indirect [SubstMap T [T]] [SubstMapCompose T T]
-  --   {k} {ℓ : List $ Action T} {σ : Subst T} (h : k = ℓ.length)
-  --   : (add T k) ∘ (ℓ ++ σ) = σ
-  -- := by subst h; simp
+  @[simp, grind <-]
+  theorem rewrite4_append_indirect [SubstMap T [T]] [SubstMapCompose T [T]]
+    {k} {ℓ : List $ Action T} {σ : Subst T} (h : k = ℓ.length)
+    : (add T k) ∘ (ℓ ++ σ) = σ
+  := by subst h; simp
 
-  -- @[grind =]
-  -- theorem subst_append_assoc {xs ys : List $ Action T} {σ : Subst T}
-  --   : xs ++ ys ++ σ = xs ++ (ys ++ σ)
-  -- := by
-  --   induction xs generalizing ys σ <;> simp [*]
+  @[grind =]
+  theorem subst_append_assoc {xs ys : List $ Action T} {σ : Subst T}
+    : xs ++ ys ++ σ = xs ++ (ys ++ σ)
+  := by
+    induction xs generalizing ys σ <;> simp [*]
 
-  -- @[grind =]
-  -- theorem subst_append_assoc_nat {xs ys : List Nat} {σ : Subst T}
-  --   : xs ++ ys ++ σ = xs ++ (ys ++ σ)
-  -- := by
-  --   induction xs generalizing ys σ <;> simp [*]
+  @[grind =]
+  theorem subst_append_assoc_nat {xs ys : List Nat} {σ : Subst T}
+    : xs ++ ys ++ σ = xs ++ (ys ++ σ)
+  := by
+    induction xs generalizing ys σ <;> simp [*]
 
-  -- @[simp]
-  -- theorem range_act_succ {s e} {σ : Subst T} : act (succ T) (s..e) ++ σ = s.succ..e.succ ++ σ := by
-  --   induction e generalizing s σ <;> simp
-  --   case _ e ih =>
-  --   simp [Ren.range]
-  --   cases Nat.decLe s e
-  --   case _ h2 => simp [ite]
-  --   case _ h2 =>
-  --     simp [ite]
-  --     cases Nat.decLe (s + 1) e
-  --     case _ h3 =>
-  --       have lem : s = e := by omega
-  --       subst lem; simp
-  --     case _ h3 =>
-  --       simp [*]
-  --       rw [subst_append_assoc, ih]; simp
-  --       rw [subst_append_assoc_nat]; simp [Ren.range]
-  --       split
-  --       case _ h4 => rw [subst_append_assoc_nat]; simp
-  --       case _ h4 => omega
+  @[simp]
+  theorem range_act_succ {s e} {σ : Subst T} : act (succ T) (s..e) ++ σ = s.succ..e.succ ++ σ := by
+    induction e generalizing s σ <;> simp
+    case _ e ih =>
+    simp [Ren.range]
+    cases Nat.decLe s e
+    case _ h2 => simp [ite]
+    case _ h2 =>
+      simp [ite]
+      cases Nat.decLe (s + 1) e
+      case _ h3 =>
+        have lem : s = e := by omega
+        subst lem; simp
+      case _ h3 =>
+        simp [*]
+        rw [subst_append_assoc, ih]; simp
+        rw [subst_append_assoc_nat]; simp [Ren.range]
+        split
+        case _ h4 => rw [subst_append_assoc_nat]; simp
+        case _ h4 => omega
 
-  -- @[simp]
-  -- theorem range_act_succ_ren {s e : Nat} {σ : Subst T}
-  --   : (s..e)⟨.succ T⟩ ++ σ = s.succ..e.succ ++ σ
-  -- := by
-  --   induction e generalizing s σ <;> simp
-  --   case _ e ih =>
-  --   simp [Ren.range]
-  --   cases Nat.decLe s e
-  --   case _ h2 => simp [ite]
-  --   case _ h2 =>
-  --     simp [ite]
-  --     cases Nat.decLe (s + 1) e
-  --     case _ h3 =>
-  --       have lem : s = e := by omega
-  --       subst lem; simp
-  --     case _ h3 =>
-  --       simp [*]
-  --       rw [subst_append_assoc_nat, ih]; simp
-  --       rw [subst_append_assoc_nat]; simp [Ren.range]
-  --       split
-  --       case _ h4 => rw [subst_append_assoc_nat]; simp
-  --       case _ h4 => omega
+  @[simp]
+  theorem range_act_succ_ren {s e : Nat} {σ : Subst T}
+    : (s..e)⟨Ren.succ T⟩ ++ σ = s.succ..e.succ ++ σ
+  := by
+    induction e generalizing s σ <;> simp
+    case _ e ih =>
+    simp [Ren.range]
+    cases Nat.decLe s e
+    case _ h2 => simp [ite]
+    case _ h2 =>
+      simp [ite]
+      cases Nat.decLe (s + 1) e
+      case _ h3 =>
+        have lem : s = e := by omega
+        subst lem; simp
+      case _ h3 =>
+        simp [*]
+        rw [subst_append_assoc_nat, ih]; simp
+        rw [subst_append_assoc_nat]; simp [Ren.range]
+        split
+        case _ h4 => rw [subst_append_assoc_nat]; simp
+        case _ h4 => omega
 
-  -- @[simp, grind =]
-  -- theorem rewrite_lift_k
-  --   [RenMap T [T]] [RenMapId T T] [RenMapCompose T T]
-  --   [SubstMap T [T]] [SubstMapId T T] [SubstMapCompose T T]
-  --   {k} {σ : Subst T}
-  --   : σ.lift k = 0..k ++ (σ ∘ +r k)
-  -- := by
-  --   induction k generalizing σ <;> simp
-  --   case _ k ih =>
-  --     rw [rewrite_lift_succ, ih]
-  --     simp; congr
+  @[simp, grind =]
+  theorem rewrite_lift_k
+    [RenMap T [T]] [RenMapId T [T]] [RenMapCompose T [T]]
+    [SubstMap T [T]] [SubstMapId T [T]] [SubstMapCompose T [T]]
+    {k} {σ : Subst T}
+    : σ.lift k = 0..k ++ (σ ∘ +r k)
+  := by
+    induction k generalizing σ <;> simp
+    case _ k ih =>
+      rw [rewrite_lift_succ, ih]
+      simp; congr
 
   -- @[simp, grind =]
   -- theorem hrewrite1 [SubstMap S T] [SubstMapId S T] {σ : Subst S} : σ ◾ (id T) = σ := by
@@ -450,122 +452,120 @@ theorem Ren.lift_eq_from_eq [RenMap T [T]] {r : Ren T} {σ : Subst T}
   -- @[simp, grind =]
   -- theorem hrewrite_lift
   --   [RenMap S S] [RenMap S T] [SubstMap S S] [SubstMap S T]
---     [RenMapId S S] [RenMapCompose S S] [SubstMapRenCommute S T]
---     {k} {σ : Subst S} {τ : Subst T}
---     : (σ ◾ τ).lift k = σ.lift k ◾ τ
---   := by
---     induction k generalizing σ τ
---     case _ => simp
---     case _ i ih =>
---       rw [rewrite_lift_succ]
---       rw [rewrite_lift_succ]
---       simp; rw [ih]
---       grind
+  --   [RenMapId S S] [RenMapCompose S S] [SubstMapRenCommute S T]
+  --   {k} {σ : Subst S} {τ : Subst T}
+  --   : (σ ◾ τ).lift k = σ.lift k ◾ τ
+  -- := by
+  --   induction k generalizing σ τ
+  --   case _ => simp
+  --   case _ i ih =>
+  --     rw [rewrite_lift_succ]
+  --     rw [rewrite_lift_succ]
+  --     simp; rw [ih]
+  --     grind
 
---   theorem hrewrite_lift1_ren
---     [RenMap S S] [SubstMap S S] [RenMap S T] [SubstMap S T] [SubstMapRenCommute S T]
---     {σ : Subst S} {τ : Ren T}
---     : (σ ◾ τ).lift = σ.lift ◾ τ
---   := by
---     simp [lift, act, SubstAction.act]; congr; funext; case _ i =>
---     cases i <;> simp [act, SubstAction.act]
---     case _ n =>
---       simp [hcompose_ren, act, SubstAction.act]
---       generalize zdef : σ.inner n = z
---       cases z <;> simp; case _ t =>
---       rw [apply_commute_ren_ren]
+  -- theorem hrewrite_lift1_ren
+  --   [RenMap S S] [SubstMap S S] [RenMap S T] [SubstMap S T] [SubstMapRenCommute S T]
+  --   {σ : Subst S} {τ : Ren T}
+  --   : (σ ◾ τ).lift = σ.lift ◾ τ
+  -- := by
+  --   simp [lift, act, SubstAction.act]; congr; funext; case _ i =>
+  --   cases i <;> simp [act, SubstAction.act]
+  --   case _ n =>
+  --     simp [hcompose_ren, act, SubstAction.act]
+  --     generalize zdef : σ.inner n = z
+  --     cases z <;> simp; case _ t =>
+  --     rw [apply_commute_ren_ren]
 
---   @[simp, grind =]
---   theorem hrewrite_lift_ren
---     [RenMap S S] [RenMap S T] [SubstMap S S] [SubstMap S T]
---     [RenMapId S S] [RenMapCompose S S] [SubstMapRenCommute S T]
---     {k} {σ : Subst S} {τ : Ren T}
---     : (σ ◾ τ).lift k = σ.lift k ◾ τ
---   := by
---     induction k generalizing σ τ
---     case _ => simp
---     case _ i ih =>
---       rw [rewrite_lift_succ]
---       rw [rewrite_lift_succ (k := i)]
---       simp; rw [ih]
--- end Subst
+  -- @[simp, grind =]
+  -- theorem hrewrite_lift_ren
+  --   [RenMap S S] [RenMap S T] [SubstMap S S] [SubstMap S T]
+  --   [RenMapId S S] [RenMapCompose S S] [SubstMapRenCommute S T]
+  --   {k} {σ : Subst S} {τ : Ren T}
+  --   : (σ ◾ τ).lift k = σ.lift k ◾ τ
+  -- := by
+  --   induction k generalizing σ τ
+  --   case _ => simp
+  --   case _ i ih =>
+  --     rw [rewrite_lift_succ]
+  --     rw [rewrite_lift_succ (k := i)]
+  --     simp; rw [ih]
+end Subst
 
--- @[grind =]
--- theorem Subst.compose_commute_succ [RenMap T [T]] {τ : Subst T}
---   : τ ∘ Ren.succ T = Ren.succ T ∘ τ.lift
--- := by congr
+@[grind =]
+theorem Subst.compose_commute_succ [RenMap T [T]] {τ : Subst T}
+  : τ ∘ Ren.succ T = Ren.succ T ∘ τ.lift
+:= by congr
 
--- @[grind =]
--- theorem Ren.compose_commute_succ {r : Ren T} : r ∘ succ T = succ T ∘ r.lift := by simp [compose]
+@[grind =]
+theorem Ren.compose_commute_succ {r : Ren T} : r ∘ succ T = succ T ∘ r.lift := by simp [compose]
 
--- theorem Subst.rewrite_lift_compose_ren_left_k1 [RenMap T [T]] {r : Ren T} {τ : Subst T}
---   : (r ∘ τ).lift = r.lift ∘ τ.lift
--- := by
---   simp [compose_ren_left, lift, Ren.lift, act, SubstAction.act]
---   funext; case _ x =>
---   cases x <;> simp
+theorem Subst.rewrite_lift_compose_ren_left_k1 [RenMap T [T]] {r : Ren T} {τ : Subst T}
+  : (r ∘ τ).lift = r.lift ∘ τ.lift
+:= by
+  simp [compose_ren_left, lift, Ren.lift, act, SubstAction.act]
+  funext; case _ x =>
+  cases x <;> simp
 
--- @[simp, grind =]
--- theorem Subst.rewrite_lift_compose_ren_left
---   [RenMap T [T]] [RenMapId T T] [RenMapCompose T T]
---   {k} {r : Ren T} {τ : Subst T}
---   : (r ∘ τ).lift k = r.lift k ∘ τ.lift k
--- := by
---   induction k generalizing r τ; congr
---   case _ k ih =>
---     rw [rewrite_lift_succ, ih]
---     rw [rewrite_lift_compose_ren_left_k1]
---     rw [<-rewrite_lift_succ]
---     rw [<-Ren.lift_of_succ]
+@[simp, grind =]
+theorem Subst.rewrite_lift_compose_ren_left
+  [RenMap T [T]] [RenMapId T [T]] [RenMapCompose T [T]]
+  {k} {r : Ren T} {τ : Subst T}
+  : (r ∘ τ).lift k = r.lift k ∘ τ.lift k
+:= by
+  induction k generalizing r τ; congr
+  case _ k ih =>
+    rw [rewrite_lift_succ, ih]
+    rw [rewrite_lift_compose_ren_left_k1]
+    rw [<-rewrite_lift_succ]
+    rw [<-Ren.lift_of_succ]
 
--- theorem Subst.lift_compose_ren_right_k1
---   [RenMap T [T]] [RenMapId T T] [RenMapCompose T T]
---   {σ : Subst T} {r : Ren T}
---   : (σ ∘ r).lift = σ.lift ∘ r.lift
--- := by
---   simp [lift, act, SubstAction.act]; congr; funext; case _ x =>
---   cases x <;> simp [act, SubstAction.act]; case _ x =>
---   simp [compose_ren_right, act, SubstAction.act]; grind
+theorem Subst.lift_compose_ren_right_k1
+  [RenMap T [T]] [RenMapId T [T]] [RenMapCompose T [T]]
+  {σ : Subst T} {r : Ren T}
+  : (σ ∘ r).lift = σ.lift ∘ r.lift
+:= by
+  simp [lift, act, SubstAction.act]; congr; funext; case _ x =>
+  cases x <;> simp [act, SubstAction.act]; case _ x =>
+  simp [compose_ren_right, Ren.compose_tuple, act, SubstAction.act]; grind
 
--- @[simp, grind =]
--- theorem Subst.lift_compose_ren_right
---   [RenMap T [T]] [RenMapId T T] [RenMapCompose T T]
---   {k} {σ : Subst T} {r : Ren T}
---   : (σ ∘ r).lift k = σ.lift k ∘ r.lift k
--- := by
---   induction k generalizing σ r; simp
---   case _ k ih =>
---     rw [rewrite_lift_succ, ih]
---     rw [lift_compose_ren_right_k1]
---     rw [<-rewrite_lift_succ]
---     rw [<-Ren.lift_of_succ]
+@[simp, grind =]
+theorem Subst.lift_compose_ren_right
+  [RenMap T [T]] [SubstMap T [T]] [RenMapId T [T]] [RenMapCompose T [T]]
+  {k} {σ : Subst T} {r : Ren T}
+  : (σ ∘ r).lift k = σ.lift k ∘ r.lift k
+:= by
+  induction k generalizing σ r; simp
+  case _ k ih =>
+    rw [rewrite_lift_succ, ih]
+    rw [lift_compose_ren_right_k1]
+    rw [<-rewrite_lift_succ]
+    rw [<-Ren.lift_of_succ]
 
--- theorem Subst.rewrite_lift_compose_k1
---   [RenMap T [T]] [SubstMap T [T]] [SubstMapRenComposeLeft T T] [SubstMapRenComposeRight T T]
---   {σ τ : Subst T}
---   : (σ ∘ τ).lift = σ.lift ∘ τ.lift
--- := by
---   simp [compose, lift, act, SubstAction.act]
---   funext; case _ x =>
---   cases x <;> simp [act, SubstAction.act]
---   case _ x =>
---   cases σ.inner x <;> simp [act, SubstAction.act]; case _ t =>
---   have lem := Subst.compose_commute_succ (τ := τ)
---   simp [lift, act, SubstAction.act] at lem
---   rw [lem]
+theorem Subst.rewrite_lift_compose_k1
+  [RenMap T [T]] [SubstMap T [T]] [SubstMapRenComposeLeft T [T]] [SubstMapRenComposeRight T [T]]
+  {σ τ : Subst T}
+  : (σ ∘ τ).lift = σ.lift ∘ τ.lift
+:= by
+  simp [compose, lift, act, SubstAction.act]
+  funext; case _ x =>
+  cases x <;> simp [act, SubstAction.act]
+  case _ x =>
+  cases σ.inner x <;> simp [act, SubstAction.act]; case _ t =>
+  simp [compose_ren_right_tuple, compose_ren_left_tuple]; congr
 
--- @[simp, grind =]
--- theorem Subst.rewrite_lift_compose
---   [RenMap T [T]] [RenMapId T T] [RenMapCompose T T] [SubstMap T [T]]
---   [SubstMapRenComposeLeft T T] [SubstMapRenComposeRight T T]
---   {k} {σ τ : Subst T}
---   : (σ ∘ τ).lift k = σ.lift k ∘ τ.lift k
--- := by
---   induction k generalizing σ τ; simp
---   case _ k ih =>
---     rw [rewrite_lift_succ, ih]
---     rw [rewrite_lift_succ (σ := σ)]
---     rw [rewrite_lift_succ (σ := τ)]
---     rw [rewrite_lift_compose_k1]
+@[simp, grind =]
+theorem Subst.rewrite_lift_compose
+  [RenMap T [T]] [RenMapId T [T]] [RenMapCompose T [T]] [SubstMap T [T]]
+  [SubstMapRenComposeLeft T [T]] [SubstMapRenComposeRight T [T]]
+  {k} {σ τ : Subst T}
+  : (σ ∘ τ).lift k = σ.lift k ∘ τ.lift k
+:= by
+  induction k generalizing σ τ; simp
+  case _ k ih =>
+    rw [rewrite_lift_succ, ih]
+    rw [rewrite_lift_succ (σ := σ)]
+    rw [rewrite_lift_succ (σ := τ)]
+    rw [rewrite_lift_compose_k1]
 
 end LeanSubst
