LeanSubst/Misc.lean
@@ -10,398 +10,397 @@ import LeanSubst.Types.List
 namespace LeanSubst
 
 universe u1 u2 u3
-variable {S : Type u1} {T : Type u2} {U : Type u3}
+variable {S : Type u1} {T T1 T2 : Type u2} {U : Type u3}
+variable {V : List (Type u2)}
 
--- instance [RenMap S T] [SubstMap S T] [SubstMapRenComposeLeft S T] : SubstMapRenComposeLeft (List S) T where
---   apply_ren_compose_left := by intro s r τ; induction s <;> simp [*]
+instance [RenMap S V] [SubstMap S V] [SubstMapRenComposeLeft S V] : SubstMapRenComposeLeft (List S) V where
+  apply_ren_compose_left := by intro s r τ; induction s <;> simp [*]
 
--- instance [RenMap S T] [RenMap T T] [SubstMap S T] [SubstMapRenComposeRight S T] : SubstMapRenComposeRight (List S) T where
---   apply_ren_compose_right := by intro s r τ; induction s <;> simp [*]
+instance [RenMap S V] [RenMapAll V] [SubstMap S V] [SubstMapRenComposeRight S V] : SubstMapRenComposeRight (List S) V where
+  apply_ren_compose_right := by intro s r τ; induction s <;> simp [*]
 
--- @[simp, grind =]
--- theorem Subst.rewrite3_cons_ren_fix [RenMap T T] [SubstMap T T] {a} {σ : Subst T} {r : Ren T}
---   : (a :: σ) ∘ r = a⟨r⟩:: (σ ∘ r)
--- := by
---   simp [cons, compose_ren_right]
---   funext; case _ x =>
---   cases x; all_goals simp [act, SubstAction.act]
+@[simp, grind =]
+theorem Subst.rewrite3_cons_ren_fix [RenMap T [T]] [SubstMap T [T]] {a} {σ : Subst T} {r : Ren T}
+  : (a :: σ) ∘ r = a⟨r⟩:: (σ ∘ r)
+:= by
+  simp [cons, compose_ren_right]
+  funext; case _ x =>
+  cases x; all_goals simp [act, SubstAction.act]
 
--- @[simp, grind =]
--- theorem Subst.rewrite3_cons_ren_subst [SubstMap T T] {x} {σ : Subst T} {r : Ren T}
---   : (x :: r) ∘ σ = σ.act x :: (r ∘ σ)
--- := by
---   simp [cons, compose_ren_left]
---   funext; case _ x =>
---   cases x; all_goals simp [act, SubstAction.act]
+@[simp, grind =]
+theorem Subst.rewrite3_cons_ren_subst [SubstMap T [T]] {x} {σ : Subst T} {r : Ren T}
+  : (x :: r) ∘ σ = σ.act x :: (r ∘ σ)
+:= by
+  simp [cons, compose_ren_left]
+  funext; case _ x =>
+  cases x; all_goals simp [act, SubstAction.act]
 
--- @[simp, grind =]
--- theorem Subst.ren_succ_beta_to {a} {r : Ren T}
---   : (r ∘ Ren.succ T) ∘ (a :: Subst.id T) = r.to
--- := by simp [compose_ren_left, Ren.to]
+@[simp, grind =]
+theorem Subst.ren_succ_beta_to {a} {r : Ren T}
+  : (r ∘ Ren.succ T) ∘ (a :: Subst.id T) = r.to
+:= by simp [compose_ren_left, Ren.to]
 
--- theorem Ren.lift_of_succ_rev {k} {r : Ren S} : r.lift (1 + k) = r.lift.lift k := by
---   induction k; simp
---   case _ k ih =>
---   rw [Ren.lift_of_succ, <-ih, <-Ren.lift_of_succ]
---   congr 1
+theorem Ren.lift_of_succ_rev {k} {r : Ren S} : r.lift (1 + k) = r.lift.lift k := by
+  induction k; simp
+  case _ k ih =>
+  rw [Ren.lift_of_succ, <-ih, <-Ren.lift_of_succ]
+  congr 1
 
--- @[grind =]
--- theorem Ren.lift_of_add {a b} {r : Ren S} : r.lift (a + b) = (r.lift a).lift b := by
---   induction a generalizing b; simp
---   case _ a ih =>
---   rw [Ren.lift_of_succ]
---   rw [<-Ren.lift_of_succ_rev]
---   rw [<-ih]; congr 1; omega
+@[grind =]
+theorem Ren.lift_of_add {a b} {r : Ren S} : r.lift (a + b) = (r.lift a).lift b := by
+  induction a generalizing b; simp
+  case _ a ih =>
+  rw [Ren.lift_of_succ]
+  rw [<-Ren.lift_of_succ_rev]
+  rw [<-ih]; congr 1; omega
 
--- @[grind =]
--- theorem Subst.compose_commute_add [RenMap T T] [SubstMap T T] [SubstMapStable T T] {k} {τ : Subst T}
---   : τ ∘ add T k = add T k ∘ τ.lift k
--- := by
---   simp [compose]; funext; case _ x =>
---   generalize zdef : τ.act x = z
---   cases z <;> simp
---   rw [apply_stable]; simp
+@[grind =]
+theorem Subst.compose_commute_add [RenMap T [T]] [SubstMap T [T]] [SubstMapStable T [T]] {k} {τ : Subst T}
+  : τ ∘ add T k = add T k ∘ τ.lift k
+:= by
+  simp [compose]; funext; case _ x =>
+  generalize zdef : τ.act x = z
+  cases z <;> simp
+  rw [SubstMapStable.apply_stable]; simp [Ren.tuple_to]
 
--- @[grind =]
--- theorem Subst.compose_commute_add_ren_subst [RenMap T T] [SubstMap T T] [SubstMapStable T T] {k} {τ : Subst T}
---   : τ ∘ Ren.add T k = Ren.add T k ∘ τ.lift k
--- := by
---   simp [compose_ren_right, compose_ren_left]
+@[grind =]
+theorem Subst.compose_commute_add_ren_subst [RenMap T [T]] [SubstMap T [T]] [SubstMapStable T [T]] {k} {τ : Subst T}
+  : τ ∘ Ren.add T k = Ren.add T k ∘ τ.lift k
+:= by
+  simp [compose_ren_right, compose_ren_left]
 
--- @[grind =]
--- theorem Subst.compose_commute_add_ren [RenMap T T] {k} {r : Ren T}
---   : r ∘ add T k = add T k ∘ r.lift k
--- := by
---   simp [compose_ren_left, compose_ren_right]
+@[grind =]
+theorem Subst.compose_commute_add_ren [RenMap T [T]] {k} {r : Ren T}
+  : r ∘ add T k = add T k ∘ r.lift k
+:= by
+  simp [compose_ren_left, compose_ren_right]
 
--- @[grind =]
--- theorem Subst.compose_commute_add_ren_ren {k} {r : Ren T}
---   : r ∘ Ren.add T k = .add T k ∘ r.lift k
--- := by simp [Ren.compose]
+@[grind =]
+theorem Subst.compose_commute_add_ren_ren {k} {r : Ren T}
+  : r ∘ Ren.add T k = .add T k ∘ r.lift k
+:= by simp [Ren.compose]
+
+@[simp]
+theorem Ren.to_cons {x} {r : Ren T} : (x::r).to = re x :: r.to := by
+  simp [to, cons, Subst.cons]; funext; case _ x =>
+  cases x <;> simp
+
+theorem Ren.cons_add_succ {T n} : n :: add T (n + 1) = add T n := by
+  induction n
+  case zero =>
+    simp [cons]
+    congr ; funext ; split <;> simp
+  case succ =>
+    simp [cons, add]
+    funext ; split <;> omega
+
+theorem Ren.assoc {T} {xs ys : List Nat} {r : Ren T} : xs ++ (ys ++ r) = xs ++ ys ++ r := by
+  induction xs <;> simp_all
+
+theorem Ren.append_range_succ_succ {T s e} {r : Ren T} {h : s ≤ e + 1} : s..(e + 2) ++ r = s..(e + 1) ++ ((e + 1) :: r) := by
+  simp_all [Ren.range, ← Ren.assoc]
+
+theorem Subst.rewrite1_append_ren_le {T s e} : s..e ++ +r e = .add T (min s e) := by
+  induction e generalizing s ; simp
+  case succ e ih =>
+    cases Nat.decLt s (e + 1)
+    case isFalse => simp_all
+    case isTrue h =>
+      cases (by omega : s ≤ e)
+      case refl => simp [Ren.cons, Ren.add] ; funext n ; split <;> grind
+      case step n _ =>
+        replace ih := @ih s
+        simp_all [Nat.min_eq_left (by omega : s ≤ n + 2)]
+        simp [Nat.min_eq_left (by omega : s ≤ n + 1)] at ih
+        rw [← ih, @Ren.append_range_succ_succ (h := (by omega : s + 1 ≤ n + 1)), Ren.cons_add_succ]
+        simp [@Ren.range_lt_cons (h := (by omega : s < n + 1))]
+
+theorem subst_append_assoc_nat {T} {xs ys : List Nat} {σ : Subst T} : xs ++ (ys ++ σ) = xs ++ ys ++ σ := by
+  induction xs <;> simp_all
+
+theorem Subst.append_range_succ_succ {T s e} {σ : Subst T} {h : s ≤ e + 1} : s..(e + 2) ++ σ = s..(e + 1) ++ ((re $ e + 1) :: σ) := by
+  simp_all [Ren.range, subst_append_assoc_nat]
+
+theorem Subst.cons_add_succ {T n} : re n :: add T (n + 1) = add T n := by
+  induction n
+  case zero =>
+    simp [cons]
+    congr ; funext n ; split <;> simp
+  case succ n _ =>
+    simp [cons, add]
+    funext ; split <;> congr 1 <;> omega
+
+theorem Subst.rewrite1_append_le {T s e} : s..e ++ +σ e = add T (min s e) := by
+  induction e generalizing s ; simp
+  case succ e ih =>
+    cases Nat.decLt s (e + 1)
+    case isFalse => simp_all
+    case isTrue h1 =>
+      cases (by omega : s ≤ e)
+      case refl => simp [Subst.cons, Subst.add] ; funext n ; split <;> grind
+      case step n _ =>
+        replace ih := @ih s
+        simp_all [Nat.min_eq_left (by omega : s ≤ n + 2)]
+        simp [Nat.min_eq_left (by omega : s ≤ n + 1)] at ih
+        rw [← ih, @Subst.append_range_succ_succ (h := (by omega : s + 1 ≤ n + 1)), cons_add_succ]
+        simp [@Ren.range_lt_cons (h := (by omega : s < n + 1))]
+
+
+@[simp, grind =]
+theorem Subst.rewrite1_append_ren {e} : 0..e ++ +r e = .id T := by
+  have lem := @rewrite1_append_ren_le T 0 e
+  simp at lem; exact lem
+
+@[simp, grind =]
+theorem Subst.rewrite1_append {e} : 0..e ++ +σ e = id T := by
+  have lem := @rewrite1_append_le T 0 e
+  simp at lem; exact lem
+
+@[simp, grind =]
+theorem Subst.rewrite_lift_ren {r : Ren T} : r.lift = 0::(r ∘ +1r) := by
+  simp [Ren.lift, Ren.cons]; funext; case _ x =>
+  cases x <;> simp
+
+@[simp, grind =]
+theorem Subst.rewrite3_append_ren_ren_cons {x} {r1 r2 : Ren T}
+  : (x::r1) ∘ r2 = r2.act x::(r1 ∘ r2)
+:= by
+  simp [Ren.cons, Ren.compose]; funext; case _ x =>
+  cases x <;> simp
+
+@[simp, grind =]
+theorem Subst.rewrite3_append_ren_ren {ℓ : List Nat} {r1 r2 : Ren T}
+  : (ℓ ++ r1) ∘ r2 = ℓ⟨r2⟩ ++ (r1 ∘ r2)
+:= by
+  induction ℓ generalizing r1 r2 <;> simp [*]
+
+@[simp]
+theorem range_act_succ_ren_fixed {s e}
+  : (s..e)⟨Ren.succ T⟩ = s.succ..e.succ
+:= by
+  induction e generalizing s; simp
+  case _ e ih =>
+    simp [Ren.range]; split <;> simp
+    case _ h =>
+    rw [ih]
+    cases Nat.decLe (s + 1) e <;> simp [ite]
+    case _ h2 =>
+      rw [Ren.range_ge_nil]; omega
+    case _ h2 =>
+      conv =>
+        lhs; simp [Ren.range]
+      split <;> simp
+
+@[simp, grind =]
+theorem Subst.rewrite_lift_k_ren {k} {r : Ren T} : r.lift k = 0..k ++ (r ∘ +r k) := by
+  induction k generalizing r <;> simp
+  case _ k ih =>
+  rw [Ren.lift_of_succ, ih]; simp
+  rw [<-Ren.compose_add_succ_right]
+
+@[simp, grind =]
+theorem Subst.rewrite4_cons_ren_add_direct {r : Ren T} {ℓ : List Nat}
+  : Ren.add T ℓ.length ∘ (ℓ ++ r) = r
+:= by simp [Ren.compose]
+
+@[simp, grind =]
+theorem Subst.rewrite4_cons_ren_add_indirect {k} {r : Ren T} {ℓ : List Nat} {h : k = ℓ.length}
+  : Ren.add T k ∘ (ℓ ++ r) = r
+:= by simp [Ren.compose, h]
+
+@[simp, grind =]
+theorem Subst.rewrite4_append_add_direct {σ : Subst T} {ℓ : List (Action T)}
+  : Ren.add T ℓ.length ∘ (ℓ ++ σ) = σ
+:= by simp [compose_ren_left]; congr
+
+@[simp, grind =]
+theorem Subst.rewrite4_append_add_indirect {k} {σ : Subst T} {ℓ : List (Action T)} {h : k = ℓ.length}
+  : Ren.add T k ∘ (ℓ ++ σ) = σ
+:= by simp [compose_ren_left, h]; congr
+
+theorem Subst.compose_ren_left_cons_lift_1 [RenMap T [T]] [SubstMap T [T]] {a : Action T} {r : Ren T} {σ : Subst T}
+  : r.lift ∘ (a :: σ) = a :: (r ∘ σ)
+:= by
+  simp; congr 1
+
+@[simp]
+theorem Subst.compose_ren_left_cons_lift_k1 [RenMap T [T]] [SubstMap T [T]] {k} {a : Action T} {r : Ren T} {σ : Subst T}
+  : r.lift (k + 1) ∘ (a :: σ) = a :: (r.lift k ∘ σ)
+:= by
+  rw [Ren.lift_of_succ, compose_ren_left_cons_lift_1]
+
+@[simp, grind =]
+theorem Subst.compose_ren_left_cons_lift_direct
+  [RenMap T [T]] [SubstMap T [T]] {ℓ : List $ Action T} {r : Ren T} {σ : Subst T}
+  : r.lift ℓ.length ∘ (ℓ ++ σ) = ℓ ++ (r ∘ σ)
+:= by
+  induction ℓ generalizing r <;> simp [-Subst.rewrite_lift_k_ren, *]
+
+@[simp, grind =]
+theorem Subst.compose_ren_left_cons_lift_indirect
+  [RenMap T [T]] [SubstMap T [T]] {k} {ℓ : List $ Action T} {r : Ren T} {σ : Subst T} {h : k = ℓ.length}
+  : r.lift k ∘ (ℓ ++ σ) = ℓ ++ (r ∘ σ)
+:= by
+  induction ℓ generalizing r <;> simp [-Subst.rewrite_lift_k_ren, *]
+
+@[simp, grind =]
+theorem Subst.compose_ren_right_append [RenMap T [T]] [SubstMap T [T]] {ℓ : List $ Action T} {r : Ren T} {σ : Subst T}
+  : (ℓ ++ σ) ∘ r = ℓ⟨r⟩ ++ σ ∘ r
+:= by
+  induction ℓ generalizing σ r <;> simp
+  case _ hd tl ih => rw [<-ih]
+
+theorem Subst.compose_ren_right_assoc
+  [RenMap S [S]] [SubstMap S [S]] [SubstMapRenComposeLeft S [S]]
+  {σ τ : Subst S} {r : Ren S}
+  : (σ ∘ r) ∘ τ = σ ∘ (r ∘ τ)
+:= by
+  simp [compose, compose_ren_left, compose_ren_right]; funext; case _ i =>
+  generalize zdef : σ.act i = z
+  cases z <;> simp
+  congr
+
+theorem Subst.compose_ren_right_assoc2
+  [RenMap S [S]] [SubstMap S [S]] [SubstMapRenComposeRight S [S]]
+  {σ τ : Subst S} {r : Ren S}
+  : (σ ∘ τ) ∘ r = σ ∘ (τ ∘ r)
+:= by
+  simp [compose, compose_ren_right]; funext; case _ i =>
+  generalize zdef : σ.act i = z
+  cases z <;> simp
+  congr
+
+-- like rewrite_lift_succ but no [RenMapId S [S]]
+theorem Subst.lift_of_succ [RenMap S [S]] [RenMapCompose S [S]] {k} {σ : Subst S} : σ.lift (k + 1) = (σ.lift k).lift := by
+  simp [lift]
+  funext n ; induction n
+  case zero => simp
+  case succ n' _  =>
+    simp
+    split <;> simp [rmap]
+    split <;> grind [Ren.add, Ren.succ, Ren.compose]
+
+theorem Subst.lift_of_succ_rev [RenMap S [S]] [RenMapCompose S [S]] {k} {σ : Subst S} : σ.lift (1 + k) = σ.lift.lift k := by
+  rw [Nat.add_comm, lift_of_succ]
+  simp [lift]
+  funext n ; induction n
+  case zero => simp [eq_comm]
+  case succ n' _ =>
+    repeat any_goals (simp ; split)
+    · simp ; omega
+    · grind [Ren.succ, Ren.add, Ren.compose]
+    · grind
+    · split <;>
+      · simp [Ren.succ, Ren.add, Ren.compose_tuple, Ren.compose] ; grind
+
+@[grind =]
+theorem Subst.lift_of_add [RenMap S [S]] [SubstMap S [S]] [RenMapId S [S]]  [RenMapCompose S [S]] {a b} {σ : Subst S} : σ.lift (a + b) = (σ.lift a).lift b := by
+  induction a generalizing σ <;> grind [lift_of_succ_rev]
 
 -- @[simp]
--- theorem Ren.to_cons {x} {r : Ren T} : (x::r).to = re x :: r.to := by
---   simp [to, cons, Subst.cons]; funext; case _ x =>
---   cases x <;> simp
-
--- theorem Ren.cons_add_succ {T n} : n :: add T (n + 1) = add T n := by
---   induction n
---   case zero =>
---     simp [cons]
---     congr ; funext ; split <;> simp
---   case succ =>
---     simp [cons, add]
---     funext ; split <;> omega
-
--- theorem Ren.assoc {T} {xs ys : List Nat} {r : Ren T} : xs ++ (ys ++ r) = xs ++ ys ++ r := by
---   induction xs <;> simp_all
-
--- theorem Ren.append_range_succ_succ {T s e} {r : Ren T} {h : s ≤ e + 1} : s..(e + 2) ++ r = s..(e + 1) ++ ((e + 1) :: r) := by
---   simp_all [Ren.range, ← Ren.assoc]
-
--- theorem Subst.rewrite1_append_ren_le {T s e} : s..e ++ +r e = .add T (min s e) := by
---   induction e generalizing s ; simp
---   case succ e ih =>
---     cases Nat.decLt s (e + 1)
---     case isFalse => simp_all
---     case isTrue h =>
---       cases (by omega : s ≤ e)
---       case refl => simp [Ren.cons, Ren.add] ; funext n ; split <;> grind
---       case step n _ =>
---         replace ih := @ih s
---         simp_all [Nat.min_eq_left (by omega : s ≤ n + 2)]
---         simp [Nat.min_eq_left (by omega : s ≤ n + 1)] at ih
---         rw [← ih, @Ren.append_range_succ_succ (h := (by omega : s + 1 ≤ n + 1)), Ren.cons_add_succ]
---         simp [@Ren.range_lt_cons (h := (by omega : s < n + 1))]
-
--- theorem subst_append_assoc_nat {T} {xs ys : List Nat} {σ : Subst T} : xs ++ (ys ++ σ) = xs ++ ys ++ σ := by
---   induction xs <;> simp_all
-
--- theorem Subst.append_range_succ_succ {T s e} {σ : Subst T} {h : s ≤ e + 1} : s..(e + 2) ++ σ = s..(e + 1) ++ ((re $ e + 1) :: σ) := by
---   simp_all [Ren.range, subst_append_assoc_nat]
-
--- theorem Subst.cons_add_succ {T n} : re n :: add T (n + 1) = add T n := by
---   induction n
---   case zero =>
---     simp [cons]
---     congr ; funext n ; split <;> simp
---   case succ n _ =>
---     simp [cons, add]
---     funext ; split <;> congr 1 <;> omega
-
--- theorem Subst.rewrite1_append_le {T s e} : s..e ++ +σ e = add T (min s e) := by
---   induction e generalizing s ; simp
---   case succ e ih =>
---     cases Nat.decLt s (e + 1)
---     case isFalse => simp_all
---     case isTrue h1 =>
---       cases (by omega : s ≤ e)
---       case refl => simp [Subst.cons, Subst.add] ; funext n ; split <;> grind
---       case step n _ =>
---         replace ih := @ih s
---         simp_all [Nat.min_eq_left (by omega : s ≤ n + 2)]
---         simp [Nat.min_eq_left (by omega : s ≤ n + 1)] at ih
---         rw [← ih, @Subst.append_range_succ_succ (h := (by omega : s + 1 ≤ n + 1)), cons_add_succ]
---         simp [@Ren.range_lt_cons (h := (by omega : s < n + 1))]
-
-
--- @[simp, grind =]
--- theorem Subst.rewrite1_append_ren {e} : 0..e ++ +r e = .id T := by
---   have lem := @rewrite1_append_ren_le T 0 e
---   simp at lem; exact lem
-
--- @[simp, grind =]
--- theorem Subst.rewrite1_append {e} : 0..e ++ +σ e = id T := by
---   have lem := @rewrite1_append_le T 0 e
---   simp at lem; exact lem
-
--- @[simp, grind =]
--- theorem Subst.rewrite_lift_ren {r : Ren T} : r.lift = 0::(r ∘ +1r) := by
---   simp [Ren.lift, Ren.cons]; funext; case _ x =>
---   cases x <;> simp
-
--- @[simp, grind =]
--- theorem Subst.rewrite3_append_ren_ren_cons {x} {r1 r2 : Ren T}
---   : (x::r1) ∘ r2 = r2.act x::(r1 ∘ r2)
--- := by
---   simp [Ren.cons, Ren.compose]; funext; case _ x =>
---   cases x <;> simp
-
--- @[simp, grind =]
--- theorem Subst.rewrite3_append_ren_ren {ℓ : List Nat} {r1 r2 : Ren T}
---   : (ℓ ++ r1) ∘ r2 = ℓ⟨r2⟩ ++ (r1 ∘ r2)
--- := by
---   induction ℓ generalizing r1 r2 <;> simp [*]
-
--- @[simp]
--- theorem range_act_succ_ren_fixed {s e}
---   : (s..e)⟨.succ T⟩ = s.succ..e.succ
--- := by
---   induction e generalizing s; simp
---   case _ e ih =>
---     simp [Ren.range]; split <;> simp
---     case _ h =>
---     rw [ih]
---     cases Nat.decLe (s + 1) e <;> simp [ite]
---     case _ h2 =>
---       rw [Ren.range_ge_nil]; omega
---     case _ h2 =>
---       conv =>
---         lhs; simp [Ren.range]
---       split <;> simp
-
--- @[simp, grind =]
--- theorem Subst.rewrite_lift_k_ren {k} {r : Ren T} : r.lift k = 0..k ++ (r ∘ +r k) := by
---   induction k generalizing r <;> simp
---   case _ k ih =>
---   rw [Ren.lift_of_succ, ih]; simp
---   rw [<-Ren.compose_add_succ_right]
-
--- @[simp, grind =]
--- theorem Subst.rewrite4_cons_ren_add_direct {r : Ren T} {ℓ : List Nat}
---   : Ren.add T ℓ.length ∘ (ℓ ++ r) = r
--- := by simp [Ren.compose]
-
--- @[simp, grind =]
--- theorem Subst.rewrite4_cons_ren_add_indirect {k} {r : Ren T} {ℓ : List Nat} {h : k = ℓ.length}
---   : Ren.add T k ∘ (ℓ ++ r) = r
--- := by simp [Ren.compose, h]
-
--- @[simp, grind =]
--- theorem Subst.rewrite4_append_add_direct {σ : Subst T} {ℓ : List (Action T)}
---   : Ren.add T ℓ.length ∘ (ℓ ++ σ) = σ
--- := by simp [compose_ren_left]; congr
-
--- @[simp, grind =]
--- theorem Subst.rewrite4_append_add_indirect {k} {σ : Subst T} {ℓ : List (Action T)} {h : k = ℓ.length}
---   : Ren.add T k ∘ (ℓ ++ σ) = σ
--- := by simp [compose_ren_left, h]; congr
-
--- theorem Subst.compose_ren_left_cons_lift_1 [RenMap T T] [SubstMap T T] {a : Action T} {r : Ren T} {σ : Subst T}
---   : r.lift ∘ (a :: σ) = a :: (r ∘ σ)
--- := by
---   simp; congr 1
-
--- @[simp]
--- theorem Subst.compose_ren_left_cons_lift_k1 [RenMap T T] [SubstMap T T] {k} {a : Action T} {r : Ren T} {σ : Subst T}
---   : r.lift (k + 1) ∘ (a :: σ) = a :: (r.lift k ∘ σ)
--- := by
---   rw [Ren.lift_of_succ, compose_ren_left_cons_lift_1]
-
--- @[simp, grind =]
--- theorem Subst.compose_ren_left_cons_lift_direct
---   [RenMap T T] [SubstMap T T] {ℓ : List $ Action T} {r : Ren T} {σ : Subst T}
---   : r.lift ℓ.length ∘ (ℓ ++ σ) = ℓ ++ (r ∘ σ)
--- := by
---   induction ℓ generalizing r <;> simp [-Subst.rewrite_lift_k_ren, *]
-
--- @[simp, grind =]
--- theorem Subst.compose_ren_left_cons_lift_indirect
---   [RenMap T T] [SubstMap T T] {k} {ℓ : List $ Action T} {r : Ren T} {σ : Subst T} {h : k = ℓ.length}
---   : r.lift k ∘ (ℓ ++ σ) = ℓ ++ (r ∘ σ)
--- := by
---   induction ℓ generalizing r <;> simp [-Subst.rewrite_lift_k_ren, *]
-
--- @[simp, grind =]
--- theorem Subst.compose_ren_right_append [RenMap T T] {ℓ : List $ Action T} {r : Ren T} {σ : Subst T}
---   : (ℓ ++ σ) ∘ r = ℓ⟨r⟩ ++ σ ∘ r
--- := by
---   induction ℓ generalizing σ r <;> simp
---   case _ hd tl ih =>
---   rw [<-ih]; simp [compose_ren_right, cons]; funext; case _ i =>
---   cases i <;> simp
-
--- theorem Subst.compose_ren_right_assoc
---   [RenMap S S] [SubstMap S S] [SubstMapRenComposeLeft S S]
---   {σ τ : Subst S} {r : Ren S}
---   : (σ ∘ r) ∘ τ = σ ∘ (r ∘ τ)
--- := by
---   simp [compose, compose_ren_left, compose_ren_right]; funext; case _ i =>
---   generalize zdef : σ.act i = z
---   cases z <;> simp
---   congr
-
--- theorem Subst.compose_ren_right_assoc2
---   [RenMap S S] [SubstMap S S] [SubstMapRenComposeRight S S]
---   {σ τ : Subst S} {r : Ren S}
---   : (σ ∘ τ) ∘ r = σ ∘ (τ ∘ r)
--- := by
---   simp [compose, compose_ren_right]; funext; case _ i =>
---   generalize zdef : σ.act i = z
---   cases z <;> simp
---   congr
-
--- -- like rewrite_lift_succ but no [RenMapId S S]
--- theorem Subst.lift_of_succ [RenMap S S] [RenMapCompose S S] {k} {σ : Subst S} : σ.lift (k + 1) = (σ.lift k).lift := by
---   simp [lift]
---   funext n ; induction n
---   case zero => simp
---   case succ n' _  =>
---     simp
---     split <;> simp [rmap]
---     split <;> grind [Ren.add, Ren.succ, Ren.compose]
-
--- theorem Subst.lift_of_succ_rev [RenMap S S] [RenMapCompose S S] {k} {σ : Subst S} : σ.lift (1 + k) = σ.lift.lift k := by
---   rw [Nat.add_comm, lift_of_succ]
---   simp [lift]
---   funext n ; induction n
---   case zero => simp [eq_comm]
---   case succ n' _ =>
---     repeat any_goals (simp ; split)
---     · simp ; omega
---     · grind [Ren.succ, Ren.add, Ren.compose]
---     · grind
---     · split <;>
---       · simp [Ren.succ, Ren.add, Ren.compose] ; grind
-
--- @[grind =]
--- theorem Subst.lift_of_add [RenMap S S] [RenMapId S S] [RenMapCompose S S] {a b} {σ : Subst S} : σ.lift (a + b) = (σ.lift a).lift b := by
---   induction a generalizing σ <;> grind [lift_of_succ_rev]
-
--- @[simp]
--- theorem Subst.ren_to_hcompose [SubstMap S T] {r : Ren S} {σ : Subst T} : r.to ◾ σ = r.to := by simp [hcompose, Ren.to]
+-- theorem Subst.ren_to_hcompose [SubstMap S V] {r : Ren S} {σ : Subst T} : r.to ◾ σ = r.to := by simp [hcompose, Ren.to]
 
 -- @[simp]
 -- theorem Subst.ren_to_hcompose_ren [RenMap S T] {r : Ren S} {k : Ren T} : r.to ◾ k = r.to := by simp [hcompose_ren, Ren.to]
 
--- @[simp]
--- theorem Subst.to_append {ℓ : List Nat} {r : Ren T} : (ℓ ++ r).to = ℓ ++ r.to := by
---   induction ℓ <;> simp_all [HAppend.hAppend, Ren.append, append_ren]
+@[simp]
+theorem Subst.to_append {ℓ : List Nat} {r : Ren T} : (ℓ ++ r).to = ℓ ++ r.to := by
+  induction ℓ <;> simp_all [HAppend.hAppend, Ren.append, append_ren]
 
--- @[simp, grind =]
--- theorem Subst.ren_rewrite1 [RenMap T T] {r : Ren T} : id T ∘ r = r.to := by simp [Ren.to, compose_ren_right]
+@[simp, grind =]
+theorem Subst.ren_rewrite1 [RenMap T [T]] {r : Ren T} : id T ∘ r = r.to := by simp [Ren.to, compose_ren_right]
 
--- @[simp, grind =]
--- theorem Subst.ren_rewrite1_left {r : Ren T} : r ∘ id T = r.to := by simp [Ren.to, compose_ren_left]
+@[simp, grind =]
+theorem Subst.ren_rewrite1_left {r : Ren T} : r ∘ id T = r.to := by simp [Ren.to, compose_ren_left]
 
--- -- Not used but maybe useful
--- theorem Subst.rmap_of_succ_smap
---   [RenMap T T] [RenMapId T T]
---   [SubstMap T T] [SubstMapCompose T T] [SubstMapRenComposeLeft T T]
---   {x : Action T} {τ : Subst T} {t : T}
---   : t⟨Ren.succ T⟩[x :: τ] = t[τ] := by simp
+-- Not used but maybe useful
+theorem Subst.rmap_of_succ_smap
+  [RenMap T [T]] [RenMapId T [T]]
+  [SubstMap T [T]] [SubstMapCompose T [T]] [SubstMapRenComposeLeft T [T]]
+  {x : Action T} {τ : Subst T} {t : T}
+  : t⟨Ren.succ T⟩[x :: τ] = t[τ] := by simp [compose_ren_left_tuple]
 
--- theorem Subst.compose_compose_left_succ
---   [RenMap T T] [RenMapId T T]
---   [SubstMap T T] [SubstMapCompose T T] [SubstMapRenComposeLeft T T]
---   {x : Action T} {σ τ : Subst T}
---   : (σ ∘ Ren.succ T) ∘ (x :: τ) = σ ∘ τ := by
---   simp [compose, smap]
---   congr ; funext n
---   generalize zdef : σ.act n = z
---   induction z <;> simp
+theorem Subst.compose_compose_left_succ
+  [RenMap T [T]] [RenMapId T [T]]
+  [SubstMap T [T]] [SubstMapCompose T [T]] [SubstMapRenComposeLeft T [T]]
+  {x : Action T} {σ τ : Subst T}
+  : (σ ∘ Ren.succ T) ∘ (x :: τ) = σ ∘ τ := by
+  simp [compose, smap]
+  congr ; funext n
+  generalize zdef : σ.act n = z
+  induction z <;> simp [compose_ren_left_tuple]
 
--- theorem Subst.compose_left_cons_lift1_indirect
---   [RenMap T T] [RenMapId T T]
---   [SubstMap T T] [SubstMapCompose T T] [SubstMapRenComposeLeft T T]
---   {x : Action T} {σ τ : Subst T}
---   : σ.lift ∘ (x :: τ) = x :: (σ ∘ τ) := by
---   rw [rewrite_lift, rewrite3_cons, Action.smap_re, cons_action0]
---   congr 1
---   exact compose_compose_left_succ
+theorem Subst.compose_left_cons_lift1_indirect
+  [RenMap T [T]] [RenMapId T [T]]
+  [SubstMap T [T]] [SubstMapCompose T [T]] [SubstMapRenComposeLeft T [T]]
+  {x : Action T} {σ τ : Subst T}
+  : σ.lift ∘ (x :: τ) = x :: (σ ∘ τ) := by
+  rw [rewrite_lift, rewrite3_cons]
+  congr 1
+  exact compose_compose_left_succ
 
--- theorem Subst.compose_left_cons_lift_indirect {k}
---   [RenMap T T] [RenMapId T T] [RenMapCompose T T]
---   [SubstMap T T] [SubstMapCompose T T] [SubstMapRenComposeLeft T T]
---   {ℓ : List $ Action T} {σ τ : Subst T} {h : k = ℓ.length}
---   : σ.lift k ∘ (ℓ ++ τ) = ℓ ++ (σ ∘ τ) := by
---   induction ℓ generalizing k <;> simp [*]
---   case cons x xs ih => rw [lift_of_succ, compose_left_cons_lift1_indirect, ← @ih xs.length rfl]
+theorem Subst.compose_left_cons_lift_indirect {k}
+  [RenMap T [T]] [RenMapId T [T]] [RenMapCompose T [T]]
+  [SubstMap T [T]] [SubstMapCompose T [T]] [SubstMapRenComposeLeft T [T]]
+  {ℓ : List $ Action T} {σ τ : Subst T} {h : k = ℓ.length}
+  : σ.lift k ∘ (ℓ ++ τ) = ℓ ++ (σ ∘ τ) := by
+  induction ℓ generalizing k <;> simp [*]
+  case cons x xs ih => rw [lift_of_succ, compose_left_cons_lift1_indirect, ← @ih xs.length rfl]
 
--- theorem Subst.compose_lift_append_indirect {k}
---   [RenMap S S] [RenMapId S S] [RenMapCompose S S]
---   [SubstMap S S] [SubstMapId S S] [SubstMapRenComposeLeft S S] [SubstMapCompose S S]
---   {ℓ1 ℓ2 : List (Action S)} (h : k = ℓ2.length)
---   : (ℓ1 ++ Subst.id S).lift k ∘ (ℓ2 ++ Subst.id S) = (ℓ2 ++ ℓ1) ++ Subst.id S := by grind [compose_left_cons_lift_indirect]
+theorem Subst.compose_lift_append_indirect {k}
+  [RenMap S [S]] [RenMapId S [S]] [RenMapCompose S [S]]
+  [SubstMap S [S]] [SubstMapId S [S]] [SubstMapRenComposeLeft S [S]] [SubstMapCompose S [S]]
+  {ℓ1 ℓ2 : List (Action S)} (h : k = ℓ2.length)
+  : (ℓ1 ++ Subst.id S).lift k ∘ (ℓ2 ++ Subst.id S) = (ℓ2 ++ ℓ1) ++ Subst.id S := by grind [compose_left_cons_lift_indirect]
 
--- @[simp]
--- theorem Subst.List.smap_append [SubstMap S T] {a b : List S} {σ : Subst T}
---   : (a ++ b)[σ] = a[σ] ++ b[σ] := by induction a <;> grind
+@[simp]
+theorem Subst.List.smap_append [SubstMap S V] {a b : List S} {σ : List.Tuple Subst V}
+  : (a ++ b)[σ,] = a[σ,] ++ b[σ,] := by induction a <;> grind
 
--- @[simp]
--- theorem Subst.List.rmap_reverse [RenMap S T] {ℓ : List S} {r : Ren T} : ℓ.reverse⟨r⟩ = ℓ⟨r⟩.reverse := by
---   induction ℓ <;> simp ; grind
+@[simp]
+theorem Subst.List.rmap_reverse [RenMap S V] {ℓ : List S} {r : List.Tuple Ren V} : ℓ.reverse⟨r,⟩ = ℓ⟨r,⟩.reverse := by
+  induction ℓ <;> simp ; grind
 
--- @[simp]
--- theorem Subst.List.smap_reverse [SubstMap S T] {ℓ : List S} {σ : Subst T} : ℓ.reverse[σ] = ℓ[σ].reverse := by
---   induction ℓ <;> simp ; grind
+@[simp]
+theorem Subst.List.smap_reverse [SubstMap S V] {ℓ : List S} {σ : List.Tuple Subst V} : ℓ.reverse[σ,] = ℓ[σ,].reverse := by
+  induction ℓ <;> simp ; grind
 
--- @[simp]
--- theorem Subst.List.rmap_map_su [RenMap T T] {ℓ : List T} {r : Ren T} : (List.map su ℓ)⟨r⟩ = List.map su ℓ⟨r⟩ := by
---   induction ℓ <;> simp ; grind
+@[simp]
+theorem Subst.List.rmap_map_su [RenMap T [T]] {ℓ : List T} {r : Ren T} : (List.map su ℓ)⟨r⟩ = List.map su ℓ⟨r⟩ := by
+  induction ℓ <;> simp ; grind
 
--- @[simp]
--- theorem Subst.List.smap_map_su [SubstMap T T] {ℓ : List T} {σ : Subst T} : (List.map su ℓ)[σ] = List.map su ℓ[σ] := by
---   induction ℓ <;> simp ; grind
+@[simp]
+theorem Subst.List.smap_map_su [SubstMap T [T]] {ℓ : List T} {σ : Subst T} : (List.map su ℓ)[σ] = List.map su ℓ[σ] := by
+  induction ℓ <;> simp ; grind
 
--- macro "subst_solve_id" : tactic => `(tactic| {
---   intro t; induction t
---   any_goals solve | simp +instances [*]
---   all_goals try simp at *; simp  +instances [*]; grind
--- })
+macro "subst_solve_id" : tactic => `(tactic| {
+  intro t; induction t
+  any_goals solve | simp +instances [*]
+  all_goals try simp at *; simp  +instances [*]; grind
+})
 
--- macro "subst_solve_stable" : tactic => `(tactic| {
---   intro r σ h
---   funext; case _ t =>
---   induction t generalizing r σ
---   all_goals
---     simp [-Subst.rewrite_lift, -Subst.rewrite_lift_k, -Subst.rewrite_lift_ren, -Subst.rewrite_lift_k_ren, *] at *
---     try simp +instances [*]
---   all_goals try solve | rw [Subst.apply_stable h]
---   all_goals try solve | (rw [<-h]; simp +instances [Ren.to])
---   all_goals try repeat funext; grind
--- })
+macro "subst_solve_stable" : tactic => `(tactic| {
+  intro r σ h
+  funext; case _ t =>
+  induction t generalizing r σ
+  all_goals
+    simp [-Subst.rewrite_lift, -Subst.rewrite_lift_k, -Subst.rewrite_lift_ren, -Subst.rewrite_lift_k_ren, *] at *
+    try simp +instances [*]
+  all_goals try solve | rw [Subst.apply_stable h]
+  all_goals try solve | (rw [<-h]; simp +instances [Ren.to])
+  all_goals try repeat funext; grind
+})
 
--- macro "subst_solve_compose" : tactic => `(tactic| {
---   intro s σ τ
---   induction s generalizing σ τ
---   any_goals solve | simp +instances [*]
---   try any_goals solve | (
---     try simp [-Subst.rewrite_lift, *]
---     try funext; case _ x =>
---     try rw [<-Ren.to_lift]
---     try simp [-Subst.rewrite_lift, *]
---     try grind)
--- })
+macro "subst_solve_compose" : tactic => `(tactic| {
+  intro s σ τ
+  induction s generalizing σ τ
+  any_goals solve | simp +instances [*]
+  try any_goals solve | (
+    try simp [-Subst.rewrite_lift, *]
+    try funext; case _ x =>
+    try rw [<-Ren.to_lift]
+    try simp [-Subst.rewrite_lift, *]
+    try grind)
+})
 
 end LeanSubst
